erasure-plugin/theories/ErasureCorrectness.v
@@ -1,0 +1,448 @@
+(* Distributed under the terms of the MIT license. *)
+From Coq Require Import Program ssreflect ssrbool.
+From MetaCoq.Common Require Import Transform config.
+From MetaCoq.Utils Require Import bytestring utils.
+From MetaCoq.PCUIC Require PCUICAst PCUICAstUtils PCUICProgram.
+From MetaCoq.SafeChecker Require Import PCUICErrors PCUICWfEnvImpl.
+From MetaCoq.Erasure Require EAstUtils ErasureFunction ErasureCorrectness EPretty Extract.
+From MetaCoq Require Import ETransform EConstructorsAsBlocks.
+From MetaCoq.Erasure Require Import EWcbvEvalNamed.
+From MetaCoq.ErasurePlugin Require Import Erasure.
+Import PCUICProgram.
+(* Import TemplateProgram (template_eta_expand).
+ *)
+Import PCUICTransform (template_to_pcuic_transform, pcuic_expand_lets_transform).
+
+(* This is the total erasure function +
+  let-expansion of constructor arguments and case branches +
+  shrinking of the global environment dependencies +
+  the optimization that removes all pattern-matches on propositions. *)
+
+Import Transform.
+
+Obligation Tactic := program_simpl.
+
+#[local] Existing Instance extraction_checker_flags.
+
+Import EWcbvEval.
+
+Lemma transform_compose_assoc
+  {program program' program'' program''' value value' value'' value''' : Type}
+  {eval : program -> value -> Prop} {eval' : program' -> value' -> Prop}
+  {eval'' : program'' -> value'' -> Prop}
+  {eval''' : program''' -> value''' -> Prop}
+  (o : t program program' value value' eval eval')
+  (o' : t program' program'' value' value'' eval' eval'')
+  (o'' : t program'' program''' value'' value''' eval'' eval''')
+  (prec : forall p : program', post o p -> pre o' p)
+  (prec' : forall p : program'', post o' p -> pre o'' p) :
+  forall x p1,
+    transform (compose o (compose o' o'' prec') prec) x p1 =
+    transform (compose (compose o o' prec) o'' prec') x p1.
+Proof.
+  cbn. intros.
+  unfold run, time.
+  f_equal. f_equal.
+  apply proof_irrelevance.
+Qed.
+
+Lemma obseq_compose_assoc
+  {program program' program'' program''' value value' value'' value''' : Type}
+  {eval : program -> value -> Prop} {eval' : program' -> value' -> Prop}
+  {eval'' : program'' -> value'' -> Prop}
+  {eval''' : program''' -> value''' -> Prop}
+  (o : t program program' value value' eval eval')
+  (o' : t program' program'' value' value'' eval' eval'')
+  (o'' : t program'' program''' value'' value''' eval'' eval''')
+  (prec : forall p : program', post o p -> pre o' p)
+  (prec' : forall p : program'', post o' p -> pre o'' p) :
+  forall x p1 p2 v1 v2, obseq (compose o (compose o' o'' prec') prec) x p1 p2 v1 v2 <->
+      obseq (compose (compose o o' prec) o'' prec') x p1 p2 v1 v2.
+Proof.
+  cbn. intros.
+  unfold run, time.
+  intros. firstorder. exists x1. split.
+  exists x0. split => //.
+  assert (correctness o' (transform o x p1)
+  (prec (transform o x p1) (correctness o x p1)) =
+  (Transform.Transform.compose_obligation_1 o o' prec x p1)). apply proof_irrelevance.
+  now rewrite -H.
+
+  exists x1. split => //.
+  exists x0. split => //.
+  assert (correctness o' (transform o x p1)
+  (prec (transform o x p1) (correctness o x p1)) =
+  (Transform.Transform.compose_obligation_1 o o' prec x p1)). apply proof_irrelevance.
+  now rewrite H.
+Qed.
+
+Import EEnvMap.GlobalContextMap.
+Lemma make_irrel Σ fr fr' : EEnvMap.GlobalContextMap.make Σ fr = EEnvMap.GlobalContextMap.make Σ fr'.
+Proof.
+  unfold make. f_equal.
+  apply proof_irrelevance.
+Qed.
+
+Lemma eval_value {efl : WcbvFlags} Σ v v' :
+  value Σ v -> eval Σ v v' -> v = v'.
+Proof.
+  intros isv ev.
+  now pose proof (eval_deterministic ev (value_final _ isv)).
+Qed.
+
+Ltac destruct_compose :=
+  match goal with
+  |- context [ transform (compose ?x ?y ?pre) ?p ?pre' ] =>
+    let pre'' := fresh in
+    let H := fresh in
+    destruct (transform_compose x y pre p pre') as [pre'' H];
+    rewrite H; clear H; revert pre''
+    (* rewrite H'; clear H'; *)
+    (* revert pre'' *)
+  end.
+
+Ltac destruct_compose_no_clear :=
+    match goal with
+    |- context [ transform (compose ?x ?y ?pre) ?p ?pre' ] =>
+      let pre'' := fresh in
+      let H := fresh in
+      destruct (transform_compose x y pre p pre') as [pre'' H];
+      rewrite H; revert pre'' H
+    end.
+
+(*
+Section TransformValue.
+  Context {program program' : Type}.
+  Context {value value' : Type}.
+  Context {eval :  program -> value -> Prop}.
+  Context {eval' : program' -> value' -> Prop}.
+  Context (t : Transform.t program program' value value' eval eval').
+
+  Lemma preserves_value p : value p.1 p.2 (transform t p)
+
+  Definition preserves_eval pre (transform : forall p : program, pre p -> program')
+      (obseq : forall p : program, pre p -> program' -> value -> value' -> Prop) :=
+      forall p v (pr : pre p),
+        eval p v ->
+        let p' := transform p pr in
+        exists v', eval' p' v' /\ obseq p pr p' v v'.
+
+    Record t :=
+    { name : string;
+
+Lemma transform_value *)
+
+
+Inductive is_construct_app : EAst.term -> Prop :=
+| is_cstr_app_cstr kn c args : Forall is_construct_app args -> is_construct_app (EAst.tConstruct kn c args)
+| is_cstr_app_app f a : is_construct_app f -> is_construct_app a -> is_construct_app (EAst.tApp f a).
+
+Section lambdabox_theorem.
+
+  Context (Σ Σ' : EEnvMap.GlobalContextMap.t) (v : EAst.term).
+
+  Context (p : pre verified_lambdabox_pipeline (Σ, v)).
+  Context (p' : pre verified_lambdabox_pipeline (Σ', v)).
+  Context (is_value : value (wfl := default_wcbv_flags) Σ v).
+
+  Lemma pres : extends_eprogram_env (Σ, v) (Σ', v) ->
+    extends_eprogram (transform verified_lambdabox_pipeline (Σ, v) p)
+        (transform verified_lambdabox_pipeline (Σ', v) p').
+  Proof.
+    epose proof (pres := verified_lambdabox_pipeline_extends).
+    red in pres. specialize (pres _ _ p p'). auto.
+  Qed.
+
+  (* Final evaluation flags *)
+  Definition evflags := {| with_prop_case := false; with_guarded_fix := false; with_constructor_as_block := true |}.
+
+  Lemma pres_firstorder_value :
+    is_construct_app v ->
+    is_construct_app (transform verified_lambdabox_pipeline (Σ, v) p).2.
+  Proof.
+    intros isapp.
+    destruct (preservation verified_lambdabox_pipeline (Σ, v) v p) as [v' [[ev] obs]].
+    { red. cbn. sq. eapply value_final, is_value. }
+    set (transp := transform _ _ p) in *.
+    assert (value (wfl := evflags) transp.1 transp.2). admit.
+    eapply eval_value in ev => //. subst v'.
+    clear -obs isapp.
+    unfold verified_lambdabox_pipeline in obs.
+    cbn [obseq compose] in obs.
+    unfold run, time in obs.
+    decompose [ex and prod] obs. clear obs. subst.
+    cbn [obseq compose verified_lambdabox_pipeline] in *.
+    cbn [obseq compose constructors_as_blocks_transformation] in *.
+    cbn [obseq run compose rebuild_wf_env_transform] in *.
+    cbn [obseq compose inline_projections_optimization] in *.
+    cbn [obseq compose remove_match_on_box_trans] in *.
+    cbn [obseq compose remove_params_optimization] in *.
+    cbn [obseq compose guarded_to_unguarded_fix] in *.
+    cbn [obseq compose verified_lambdabox_pipeline] in *.
+    subst.
+    cbn [transform rebuild_wf_env_transform] in *.
+    cbn [transform constructors_as_blocks_transformation] in *.
+    cbn [transform inline_projections_optimization] in *.
+    cbn [transform remove_match_on_box_trans] in *.
+    cbn [transform remove_params_optimization] in *.
+    cbn [transform guarded_to_unguarded_fix] in *.
+    clearbody transp. revert b. intros ->. clear transp.
+    induction isapp.
+    cbn in *. constructor. constructor.
+  Admitted.
+
+
+End lambdabox_theorem.
+
+
+Lemma rebuild_wf_env_irr {efl : EWellformed.EEnvFlags} p wf p' wf' :
+  p.1 = p'.1 ->
+  (rebuild_wf_env p wf).1 = (rebuild_wf_env p' wf').1.
+Proof.
+  destruct p as [], p' as [].
+  cbn. intros <-.
+  unfold make. f_equal. apply proof_irrelevance.
+Qed.
+
+Lemma obseq_lambdabox (Σt Σ'v : EProgram.eprogram_env) pr pr' p' v' :
+  EGlobalEnv.extends Σ'v.1 Σt.1 ->
+  obseq verified_lambdabox_pipeline Σt pr p' Σ'v.2 v' ->
+  (transform verified_lambdabox_pipeline Σ'v pr').2 = v'.
+Proof.
+  intros ext obseq.
+  destruct Σt as [Σ t], Σ'v as [Σ' v].
+  pose proof verified_lambdabox_pipeline_extends.
+  red in H.
+  assert (pr'' : pre verified_lambdabox_pipeline (Σ, v)).
+  { clear -pr pr' ext. destruct pr as [[] ?], pr' as [[] ?].
+    split. red; cbn. split => //.
+    eapply EWellformed.extends_wellformed; tea.
+    split. apply H1. cbn. destruct H4; cbn in *.
+    eapply EEtaExpandedFix.isEtaExp_expanded.
+    eapply EEtaExpandedFix.isEtaExp_extends; tea.
+    now eapply EEtaExpandedFix.expanded_isEtaExp. }
+  destruct (H _ _ pr' pr'') as [ext' ->].
+  split => //.
+  clear H.
+  move: obseq.
+  unfold verified_lambdabox_pipeline.
+  repeat destruct_compose.
+  cbn [transform rebuild_wf_env_transform] in *.
+  cbn [transform constructors_as_blocks_transformation] in *.
+  cbn [transform inline_projections_optimization] in *.
+  cbn [transform remove_match_on_box_trans] in *.
+  cbn [transform remove_params_optimization] in *.
+  cbn [transform guarded_to_unguarded_fix] in *.
+  intros ? ? ? ? ? ? ?.
+  unfold run, time.
+  cbn [obseq compose constructors_as_blocks_transformation] in *.
+  cbn [obseq run compose rebuild_wf_env_transform] in *.
+  cbn [obseq compose inline_projections_optimization] in *.
+  cbn [obseq compose remove_match_on_box_trans] in *.
+  cbn [obseq compose remove_params_optimization] in *.
+  cbn [obseq compose guarded_to_unguarded_fix] in *.
+  intros obs.
+  decompose [ex and prod] obs. clear obs. subst.
+  unfold run, time.
+  unfold transform_blocks_program. cbn [snd]. f_equal.
+  repeat destruct_compose.
+  intros.
+  cbn [transform rebuild_wf_env_transform] in *.
+  cbn [transform constructors_as_blocks_transformation] in *.
+  cbn [transform inline_projections_optimization] in *.
+  cbn [transform remove_match_on_box_trans] in *.
+  cbn [transform remove_params_optimization] in *.
+  cbn [transform guarded_to_unguarded_fix] in *.
+  eapply rebuild_wf_env_irr.
+  unfold EInlineProjections.optimize_program. cbn [fst snd].
+  f_equal.
+  eapply rebuild_wf_env_irr.
+  unfold EOptimizePropDiscr.remove_match_on_box_program. cbn [fst snd].
+  f_equal.
+  now eapply rebuild_wf_env_irr.
+Qed.
+
+Lemma extends_erase_pcuic_program {guard : abstract_guard_impl} (Σ : global_env_ext_map) t t' nin nin' nin0 nin0' wf wf' ty ty' :
+  PCUICWcbvEval.eval Σ t' t ->
+  EGlobalEnv.extends
+    (@erase_pcuic_program guard (Σ, t) nin nin' wf ty).1
+    (@erase_pcuic_program guard (Σ, t') nin0 nin0' wf' ty').1.
+Proof.
+  intros ev.
+  cbn.
+  unfold ErasureFunction.erase_global_fast.
+  set (eg := ErasureFunction.erase _ _ _ _ _).
+  set (eg' := ErasureFunction.erase _ _ _ _ _).
+  erewrite ErasureFunction.erase_global_deps_fast_spec.
+  erewrite ErasureFunction.erase_global_deps_fast_spec.
+  epose proof ErasureFunction.erase_global_decls_irr.
+Admitted.
+
+Section pipeline_theorem.
+
+  Fixpoint compile_value_box (t : PCUICAst.term) (acc : list EAst.term) : EAst.term :=
+    match t with
+    | PCUICAst.tApp f a => compile_value_box f (acc ++ [compile_value_box a []])
+    | PCUICAst.tConstruct i n _ => EAst.tConstruct i n acc
+    | _ => EAst.tVar "error"
+    end.
+
+  Instance cf : checker_flags := extraction_checker_flags.
+  Instance nf : PCUICSN.normalizing_flags := PCUICSN.extraction_normalizing.
+
+  Variable Σ : global_env_ext_map.
+  Variable HΣ : PCUICTyping.wf_ext Σ.
+  Variable expΣ : PCUICEtaExpand.expanded_global_env Σ.1.
+
+  Variable t : PCUICAst.term.
+  Variable expt : PCUICEtaExpand.expanded Σ.1 [] t.
+
+  Variable v : PCUICAst.term.
+
+  Variable i : Kernames.inductive.
+  Variable u : Universes.Instance.t.
+  Variable args : list PCUICAst.term.
+
+  Variable typing : PCUICTyping.typing Σ [] t (PCUICAst.mkApps (PCUICAst.tInd i u) args).
+
+  Variable fo : @PCUICFirstorder.firstorder_ind Σ (PCUICFirstorder.firstorder_env Σ) i.
+
+  Variable Normalisation :  PCUICSN.NormalizationIn Σ.
+
+  Lemma precond : pre verified_erasure_pipeline (Σ, t).
+  Proof.
+    hnf. repeat eapply conj; sq; cbn; eauto.
+    - red. cbn. eauto.
+    - todo "normalization".
+    - todo "normalization".
+  Qed.
+
+  Variable Heval : ∥PCUICWcbvEval.eval Σ t v∥.
+
+  Lemma precond2 : pre verified_erasure_pipeline (Σ, v).
+  Proof.
+    cbn.  repeat eapply conj; sq; cbn; eauto.
+    - red. cbn. split; eauto.
+      eexists.
+      eapply PCUICClassification.subject_reduction_eval; eauto.
+    - todo "preservation of eta expandedness".
+    - todo "normalization".
+    - todo "normalization".
+  Qed.
+
+  Let Σ_t := (transform verified_erasure_pipeline (Σ, t) precond).1.
+  Let t_t := (transform verified_erasure_pipeline (Σ, t) precond).2.
+  Let v_t := compile_value_box v [].
+
+  Lemma fo_v : PCUICFirstorder.firstorder_value Σ [] v.
+  Proof.
+    sq.
+    eapply PCUICFirstorder.firstorder_value_spec; eauto.
+    - eapply PCUICClassification.subject_reduction_eval; eauto.
+    - eapply PCUICWcbvEval.eval_to_value; eauto.
+  Qed.
+
+
+  Lemma v_t_spec : v_t = (transform verified_erasure_pipeline (Σ, v) precond2).2.
+  Proof.
+    unfold v_t. generalize fo_v, precond2. clear.
+    induction 1.
+    intros. unfold verified_erasure_pipeline.
+    repeat destruct_compose. intros.
+    cbn [transform erase_transform].
+    cbn [transform pcuic_expand_lets_transform].
+  Admitted.
+
+  Import PCUICWfEnv.
+
+
+
+  Lemma verified_erasure_pipeline_theorem :
+    ∥ eval (wfl := extraction_wcbv_flags) Σ_t t_t v_t∥.
+  Proof.
+    hnf.
+    pose proof (preservation verified_erasure_pipeline (Σ, t)) as Hcorr.
+    unshelve eapply Hcorr in Heval as Hev. eapply precond.
+    destruct Hev as [v' [[H1] H2]].
+    move: H2.
+
+    (* repeat match goal with
+      [ H : obseq _ _ _ _ _ |- _ ] => hnf in H ;  decompose [ex and prod] H ; subst
+    end. *)
+    rewrite v_t_spec.
+    subst v_t Σ_t t_t.
+    revert H1.
+    unfold verified_erasure_pipeline.
+    intros.
+    revert H1 H2. clear Hcorr.
+    intros ev obs.
+    cbn [obseq compose] in obs.
+    unfold run, time in obs.
+    decompose [ex and prod] obs. clear obs.
+    subst.
+    cbn [obseq compose erase_transform] in *.
+    cbn [obseq compose pcuic_expand_lets_transform] in *.
+    subst.
+    move: ev b.
+    repeat destruct_compose.
+    intros.
+    move: b.
+    cbn [transform rebuild_wf_env_transform] in *.
+    cbn [transform constructors_as_blocks_transformation] in *.
+    cbn [transform inline_projections_optimization] in *.
+    cbn [transform remove_match_on_box_trans] in *.
+    cbn [transform remove_params_optimization] in *.
+    cbn [transform guarded_to_unguarded_fix] in *.
+    cbn [transform erase_transform] in *.
+    cbn [transform compose pcuic_expand_lets_transform] in *.
+    unfold run, time.
+    cbn [obseq compose constructors_as_blocks_transformation] in *.
+    cbn [obseq run compose rebuild_wf_env_transform] in *.
+    cbn [obseq compose inline_projections_optimization] in *.
+    cbn [obseq compose remove_match_on_box_trans] in *.
+    cbn [obseq compose remove_params_optimization] in *.
+    cbn [obseq compose guarded_to_unguarded_fix] in *.
+    cbn [obseq compose erase_transform] in *.
+    cbn [obseq compose pcuic_expand_lets_transform] in *.
+    cbn [transform compose pcuic_expand_lets_transform] in *.
+    cbn [transform erase_transform] in *.
+    destruct Heval.
+    pose proof typing as typing'.
+    eapply PCUICClassification.subject_reduction_eval in typing'; tea.
+    eapply PCUICExpandLetsCorrectness.pcuic_expand_lets in typing'.
+    rewrite PCUICExpandLetsCorrectness.trans_mkApps /= in typing'.
+    destruct H1.
+    (* pose proof (abstract_make_wf_env_ext) *)
+    unfold PCUICExpandLets.expand_lets_program.
+    set (em := build_global_env_map _).
+    unfold erase_program.
+    set (f := map_squash _ _). cbn in f.
+    destruct H. destruct s as [[]].
+    set (wfe := build_wf_env_from_env em (map_squash (PCUICTyping.wf_ext_wf (em, Σ.2)) (map_squash fst (conj (sq (w0, s)) a).p1))).
+    destruct Heval.
+    eapply (ErasureFunction.firstorder_erases_deterministic optimized_abstract_env_impl wfe Σ.2) in b0. 3:tea.
+    2:{ cbn. reflexivity. }
+    2:{ eapply PCUICExpandLetsCorrectness.trans_wcbveval. eapply PCUICWcbvEval.eval_closed; tea. apply HΣ.
+        admit.
+        eapply PCUICWcbvEval.value_final. now eapply PCUICWcbvEval.eval_to_value in X0. }
+    2:{ clear -fo. admit. }
+    2:{ apply HΣ. }
+    2:{ apply PCUICExpandLetsCorrectness.trans_wf, HΣ. }
+    rewrite b0.
+    intros obs.
+    constructor.
+    match goal with [ H1 : eval _ _ ?v1 |- eval _ _ ?v2 ] => enough (v2 = v1) as -> by exact ev end.
+    eapply obseq_lambdabox; revgoals.
+    unfold erase_pcuic_program. cbn [fst snd]. exact obs.
+    clear obs b0 ev e w.
+    eapply extends_erase_pcuic_program. cbn.
+    eapply (PCUICExpandLetsCorrectness.trans_wcbveval (Σ := (Σ.1, Σ.2))). admit. exact X0.
+  Admitted.
+
+  Lemma verified_erasure_pipeline_lambda :
+    PCUICAst.isLambda t -> EAst.isLambda t_t.
+  Proof.
+    unfold t_t. clear.
+  Admitted.
+
+End pipeline_theorem.
